Prove preserving_compiler transitivity

src/named/CompilerTransitivity.v
@@ -38,154 +38,437 @@ Section CompileFn.
     case_match; basic_core_crush.
   Qed.
   Hint Rewrite lookup_cmp_distributes : lang_core.
-
   
-  Lemma compile_cmp_distributes src ir tgt cmp' e
-    : all_fresh ir ->
-      ws_lang tgt ->
-      preserving_compiler tgt cmp ir ->
-      preserving_compiler ir cmp' src ->
-      forall c t, wf_term src c e t ->
-      (compile (compile_cmp cmp') e)
-      = (compile cmp (compile cmp' e)).
-  Proof.
-    intros frsrc wstgt pres_cmp pres_cmp'.
-    induction e; basic_goal_prep; basic_core_crush.
-    symmetry.
-    case_match; simpl.
-    2:admit (*TODO:contradiction*).
-    case_match; simpl.
-    2:admit (*TODO: contradiction w/ term*).
-    erewrite compile_term_subst; unfold ws_lang; eauto.
-    2: admit (*TODO: use term_case_in_wf lemma (write if it doesn't exist)*).
-    {
-      rewrite compile_subst_combine.
-      rewrite map_map.
-      f_equal.
-      f_equal.
-      (*TODO: need separate lemma*)
-      assert (exists c', wf_args src c l c') by admit; clear H0.
-      firstorder.
-      revert dependent x.
-      
-      revert dependent l; induction l; destruct x; basic_goal_prep; firstorder auto;
-        inversion H0; subst; clear H0.
-      f_equal; eauto.
+  Fixpoint term_in_cmp_domain e :=
+    match e with
+    | var _ => True
+    | con n s =>
+      (exists args e, In (n,term_case args e) cmp /\ length args = length s) /\
+      all term_in_cmp_domain s
+    end.
 
-      erewrite H; eauto.
+  Definition sort_in_cmp_domain t :=
+    match t with
+    | scon n s =>
+      (exists args e, In (n,sort_case args e) cmp /\ length args = length s) /\
+      all term_in_cmp_domain s
+    end.
+    
+End CompileFn.
+
+
+(*TODO: move to utils*)
+Lemma all_fresh_named_map A B l (f : A -> B)
+  : all_fresh (named_map f l) <-> all_fresh l.
+Proof.
+  induction l; basic_goal_prep; basic_utils_crush.
+Qed.
+Hint Rewrite all_fresh_named_map : utils.
+
+(*TODO: move to utils*)
+Lemma map_fst_combine A B (l1 : list A) (l2 : list B)
+  : length l1 = length l2 ->
+    map fst (combine l1 l2) = l1.
+Proof.
+  revert l2; induction l1; destruct l2;
+    basic_goal_prep;
+    basic_utils_crush.
+Qed.
+Hint Rewrite map_fst_combine : utils.
+
+
+(*TODO: move to utils*)
+Lemma named_map_combine A B (f : A -> B) l1 l2
+  : named_map f (combine l1 l2) = combine l1 (map f l2).
+Proof.
+  revert l2; induction l1; destruct l2;
+    basic_goal_prep;
+    basic_utils_crush.
+Qed.
+Hint Rewrite named_map_combine : utils.
+
+(*TODO: move to Compilers.v*)
+Definition ws_ccase cc :=
+  match cc with
+  | term_case args e => well_scoped args e
+  | sort_case args e => well_scoped args e
+  end.
+
+
+Lemma in_ws_term_cmp n args e cmp
+  : all ws_ccase (map snd cmp) ->
+    In (n:string, term_case args e) cmp ->
+    well_scoped args e.
+Proof.
+  induction cmp; basic_goal_prep; basic_core_crush.
+Qed.
+
+
+Lemma in_ws_sort_cmp n args e cmp
+  : all ws_ccase (map snd cmp) ->
+    In (n:string, sort_case args e) cmp ->
+    well_scoped args e.
+Proof.
+  induction cmp; basic_goal_prep; basic_core_crush.
+Qed.
+
+(*TODO: replace Compilers.v versions with these;
+  might help with inductive_implies_semantic last induction?
+ *)
+
+Lemma compile_term_subst cmp e s
+  : all_fresh cmp ->
+    all ws_ccase (map snd cmp) ->
+    term_in_cmp_domain cmp e ->
+    well_scoped (map fst s) e ->
+    compile cmp e[/s/] = (compile cmp e)[/compile_subst cmp s/].
+Proof.
+  intros allfcmp all_ws.
+  induction e; basic_goal_prep; basic_core_crush.
+  case_match; simpl; eauto.
+  apply named_list_lookup_err_in in HeqH4.
+  pose proof (in_all_fresh_same _ _ _ _ allfcmp H0 HeqH4).
+  subst.
+
+  rewrite subst_assoc.
+  2:{
+    basic_core_crush.
+    eapply in_ws_term_cmp; eauto.
+  }
+  f_equal.
+  unfold subst_cmp.
+  basic_utils_crush.
+  f_equal.
+
+  (*prove inner induction*)
+  clear x x0 H0 H2 HeqH4.
+  revert dependent l.
+  induction l; basic_goal_prep; basic_core_crush.
+Qed.
+Hint Rewrite compile_term_subst : lang_core.
+
+
+Lemma compile_args_subst cmp e s
+  : all_fresh cmp ->
+    all ws_ccase (map snd cmp) ->
+    all (term_in_cmp_domain cmp) e ->
+    well_scoped (map fst s) e ->
+    compile_args cmp e[/s/] = (compile_args cmp e)[/compile_subst cmp s/].
+Proof.
+  induction e; basic_goal_prep; basic_core_crush.
+Qed.
+
+Lemma compile_sort_subst cmp e s
+  : all_fresh cmp ->
+    all ws_ccase (map snd cmp) ->
+    sort_in_cmp_domain cmp e ->
+    well_scoped (map fst s) e ->
+    compile_sort cmp e[/s/] = (compile_sort cmp e)[/compile_subst cmp s/].
+Proof.
+  intros allfcmp all_ws.
+  induction e; basic_goal_prep; basic_core_crush.
+  case_match; simpl; eauto.
+  apply named_list_lookup_err_in in HeqH3.
+  pose proof (in_all_fresh_same _ _ _ _ allfcmp H HeqH3).
+  subst.
+
+  rewrite subst_assoc.
+  2:{
+    basic_core_crush.
+    eapply in_ws_sort_cmp; eauto.
+  }
+  f_equal.
+  unfold subst_cmp.
+  basic_utils_crush.
+  f_equal.
+  apply compile_args_subst; eauto.
+Qed.
+Hint Rewrite compile_sort_subst : lang_core.
+
+Definition ccase_in_cmp_domain cmp cc :=
+  match cc with
+  | term_case _ e => term_in_cmp_domain cmp e
+  | sort_case _ e => sort_in_cmp_domain cmp e
+  end.
+
+(* TODO: move to utils*)
+Lemma pair_in_map_snd {A B} (a:A) (b:B) l
+  : In (a,b) l -> In b (map snd l).
+Proof.
+  induction l; basic_goal_prep; basic_utils_crush.
+Qed.
+#[export] Hint Resolve pair_in_map_snd : utils.
+
+Lemma compile_cmp_distributes cmp cmp' e
+  : all ws_ccase (map snd cmp) ->
+    all_fresh cmp ->
+    all ws_ccase (map snd cmp') ->
+    all_fresh cmp' ->
+    all (ccase_in_cmp_domain cmp) (map snd cmp') ->
+    term_in_cmp_domain cmp' e ->
+    (compile (compile_cmp cmp cmp') e)
+    = (compile cmp (compile cmp' e)).
+Proof.
+  intros all_ws_cmp allfr_cmp all_ws_cmp' allfr_cmp' cmp'_in_dom.
+  induction e; basic_goal_prep; basic_core_crush.
+  assert (Some (term_case x x0) = named_list_lookup_err cmp' n).
+  {
+    rewrite all_fresh_named_list_lookup_err_in; eauto.
+  }
+  rewrite <- H3.
+  assert (Some (term_case x (compile cmp x0))
+          = named_list_lookup_err (compile_cmp cmp cmp') n).
+  {
+    rewrite all_fresh_named_list_lookup_err_in.
+    2: unfold compile_cmp; basic_utils_crush.
+    rewrite all_fresh_named_list_lookup_err_in in H3; eauto.
+    unfold compile_cmp.
+    change (term_case x (compile cmp x0))
+      with (compile_ccase cmp (term_case x x0)).
+    eapply in_named_map; eauto.
+  }
+  rewrite <- H4.
+  erewrite compile_term_subst; unfold ws_lang;eauto.
+
+  {
+    f_equal.
+    unfold compile_subst.
+    autorewrite with utils.
+    f_equal.
+    
+
+    (*nested induction*)
+    clear x x0 H0 H1 H3 H4.
+    revert dependent l.
+    induction l; basic_goal_prep; basic_core_crush.
+  }
+  {
+    assert  (ccase_in_cmp_domain cmp (term_case x x0)).
+    {
+      eapply in_all; eauto.
+      eauto with utils.
     }
-    admit (*TODO: combine_map_fst*).
-  Admitted.
+    repeat autorewrite with utils; auto.
+  }
+  repeat autorewrite with utils; auto.
+  eapply in_ws_term_cmp; [|eauto]; eauto.
+Qed.
+Hint Rewrite compile_cmp_distributes : lang_core.
 
-  
-  Lemma compile_args_cmp_distributes src ir tgt cmp' e
-    : all_fresh ir ->
-      ws_lang tgt ->
-      preserving_compiler tgt cmp ir ->
-      preserving_compiler ir cmp' src ->
-      forall c c', wf_args src c e c'->
-      (compile_args (compile_cmp cmp') e)
-      = (compile_args cmp (compile_args cmp' e)).
-  Proof.
-     intros frsrc wstgt pres_cmp pres_cmp'.
-     induction e; basic_goal_prep; basic_core_crush.
 
-     {
-       inversion H; subst; clear H.
-       eapply compile_cmp_distributes; [| | eauto | eauto | ..];
-         unfold ws_lang; eauto.
-     }
-     {
-       inversion H; subst; clear H.
-       eauto.
-     }
-  Qed.
+Lemma compile_args_cmp_distributes cmp cmp' e
+  : all ws_ccase (map snd cmp) ->
+    all_fresh cmp ->
+    all ws_ccase (map snd cmp') ->
+    all_fresh cmp' ->
+    all (ccase_in_cmp_domain cmp) (map snd cmp') ->
+    all (term_in_cmp_domain cmp') e ->
+    (compile_args (compile_cmp cmp cmp') e)
+    = (compile_args cmp (compile_args cmp' e)).
+Proof.
+  intros all_ws_cmp allfr_cmp all_ws_cmp' allfr_cmp' cmp'_in_dom.
+  induction e; basic_goal_prep; basic_core_crush.
+Qed.
+Hint Rewrite compile_args_cmp_distributes : lang_core.
+
+
+Lemma compile_sort_cmp_distributes cmp cmp' e
+  : all ws_ccase (map snd cmp) ->
+    all_fresh cmp ->
+    all ws_ccase (map snd cmp') ->
+    all_fresh cmp' ->
+    all (ccase_in_cmp_domain cmp) (map snd cmp') ->
+    sort_in_cmp_domain cmp' e ->
+    (compile_sort (compile_cmp cmp cmp') e)
+    = (compile_sort cmp (compile_sort cmp' e)).
+Proof.
+  intros all_ws_cmp allfr_cmp all_ws_cmp' allfr_cmp' cmp'_in_dom.
+  destruct e; basic_goal_prep; basic_core_crush.
+  assert (Some (sort_case x x0) = named_list_lookup_err cmp' s).
+  {
+    rewrite all_fresh_named_list_lookup_err_in; eauto.
+  }
+  rewrite <- H2.
+  assert (Some (sort_case x (compile_sort cmp x0))
+          = named_list_lookup_err (compile_cmp cmp cmp') s).
+  {
+    rewrite all_fresh_named_list_lookup_err_in.
+    2: unfold compile_cmp; basic_utils_crush.
+    rewrite all_fresh_named_list_lookup_err_in in H2; eauto.
+    unfold compile_cmp.
+    change (sort_case x (compile_sort cmp x0))
+      with (compile_ccase cmp (sort_case x x0)).
+    eapply in_named_map; eauto.
+  }
+  rewrite <- H3.
+  erewrite compile_sort_subst; unfold ws_lang;eauto.
+
+  {
+    f_equal.
+    unfold compile_subst.
+    autorewrite with utils.
+    f_equal.
     
-  Lemma compile_sort_cmp_distributes src ir tgt cmp' e
-    : all_fresh ir ->
-      ws_lang tgt ->
-      preserving_compiler tgt cmp ir ->
-      preserving_compiler ir cmp' src ->
-      forall c, wf_sort src c e ->
-      (compile_sort (compile_cmp cmp') e)
-      = (compile_sort cmp (compile_sort cmp' e)).
-  Proof.
-    intros frsrc wstgt pres_cmp pres_cmp'.
-    destruct e; basic_goal_prep; basic_core_crush.
-    symmetry.
-    case_match; simpl.
-    2:admit (*TODO:contradiction*).
-    case_match; simpl.
-    admit (*TODO: contradiction w/ term*).
-    erewrite compile_sort_subst; unfold ws_lang; eauto.
-    2: admit (*TODO: use term_case_in_wf lemma (write if it doesn't exist)*).
+
+    (*nested induction*)
+    clear x x0 H0 H H2 H3.
+    revert dependent l.
+    induction l; basic_goal_prep; basic_core_crush.
+  }
+  {
+    assert  (ccase_in_cmp_domain cmp (sort_case x x0)).
     {
-      rewrite compile_subst_combine.
-      rewrite map_map.
-      f_equal.
-      f_equal.
-      (*TODO: need separate lemma*)
-      assert (exists c', wf_args src c l c') by admit; clear H0.
-      firstorder.
-      pose proof  compile_args_cmp_distributes  as p.
-      unfold compile_args in p.
-      erewrite p; eauto.
-      rewrite map_map; eauto.
+      eapply in_all; eauto.
+      eauto with utils.
+    }
+    repeat autorewrite with utils; auto.
+  }
+  repeat autorewrite with utils; auto.
+  eapply in_ws_sort_cmp; [|eauto]; eauto.
+Qed.
+Hint Rewrite compile_sort_cmp_distributes : lang_core.
 
-      split; auto.
-      admit (*TODO: should be somewhere in the context*).
-  Admitted.
 
-  
-  Lemma compile_ctx_cmp_distributes src ir tgt cmp' c
-    : all_fresh ir ->
-      ws_lang tgt ->
-      preserving_compiler tgt cmp ir ->
-      preserving_compiler ir cmp' src ->
-      wf_ctx src c ->
-      (compile_ctx (compile_cmp cmp') c)
-      = (compile_ctx cmp (compile_ctx cmp' c)).
-  Proof.
-    intros frsrc wstgt pres_cmp pres_cmp'.
-    induction 1; basic_goal_prep; basic_core_crush.
-    f_equal; eauto.
-    erewrite compile_sort_cmp_distributes; [| | | eauto | eauto |..];
-      eauto.
-    unfold ws_lang; split; eauto.
-  Qed.
-    
-  
-  Theorem preservation_transitivity src ir tgt cmp'
-    : wf_lang src ->
-      wf_lang ir ->
-      wf_lang tgt ->
-      preserving_compiler tgt cmp ir ->
-      preserving_compiler ir cmp' src ->
-      preserving_compiler tgt (compile_cmp cmp') src.
-  Proof using .
-    intros wfsrc wfir wftgt pres_cmp pres_cmp'.
-    pose proof (inductive_implies_semantic wfir wftgt pres_cmp).
+Lemma compile_ctx_cmp_distributes cmp cmp' e
+  : all ws_ccase (map snd cmp) ->
+    all_fresh cmp ->
+    all ws_ccase (map snd cmp') ->
+    all_fresh cmp' ->
+    all (ccase_in_cmp_domain cmp) (map snd cmp') ->
+    all (sort_in_cmp_domain cmp') (map snd e) ->
+    (compile_ctx (compile_cmp cmp cmp') e)
+    = (compile_ctx cmp (compile_ctx cmp' e)).
+Proof.
+  intros all_ws_cmp allfr_cmp all_ws_cmp' allfr_cmp' cmp'_in_dom.
+  induction e; basic_goal_prep; basic_core_crush.
+Qed.
+Hint Rewrite compile_ctx_cmp_distributes : lang_core.   
+
+
+Lemma preserving_is_well_scoped tgt cmp ir
+  : ws_lang tgt ->
+    preserving_compiler tgt cmp ir ->
+    all ws_ccase (map snd cmp).
+Proof.
+  induction 2; basic_goal_prep; intuition;
+    replace (map fst c) with (map fst (compile_ctx cmp c)).
+  eapply wf_sort_implies_ws; eauto.
+  apply named_map_fst_eq; eauto.
+  eapply wf_term_implies_ws; eauto.
+  apply named_map_fst_eq; eauto.
+Qed.
+#[export] Hint Resolve preserving_is_well_scoped : lang_core.
+
+
+Lemma sort_in_preserving_lang_in_cmp tgt cmp src n c' args
+  : preserving_compiler tgt cmp src ->
+    In (n, sort_rule c' args) src ->
+    exists t, In (n, sort_case (map fst c') t) cmp.
+Proof.
+  induction 1; basic_goal_prep;
+    basic_core_crush.
+Qed.
+
+Lemma term_in_preserving_lang_in_cmp tgt cmp src n c' args t
+  : preserving_compiler tgt cmp src ->
+    In (n, term_rule c' args t) src ->
+    exists e, In (n, term_case (map fst c') e) cmp.
+Proof.
+  induction 1; basic_goal_prep;
+    basic_core_crush.
+Qed.
+
+
+
+Lemma wf_in_domain tgt cmp src
+  : preserving_compiler tgt cmp src ->    
+    (forall c t,
+        wf_sort src c t ->
+        sort_in_cmp_domain cmp t)
+    /\ (forall c e t,
+           wf_term src c e t ->
+           term_in_cmp_domain cmp e)
+    /\ (forall c s' c',
+           wf_args src c s' c' ->
+           all (term_in_cmp_domain cmp) s').
+Proof.
+  intro pres_cmp.
+  apply wf_judge_ind; basic_goal_prep;
+    basic_core_crush.
+  {
+    pose proof (sort_in_preserving_lang_in_cmp _ _ _ pres_cmp H).
     firstorder.
-    revert wfsrc.
-    induction pres_cmp'; basic_goal_prep; constructor;
-      autorewrite with lang_core in *; firstorder eauto.
+    exists (map fst c').
+    exists x.
+    basic_core_crush.
+  }
+  {
+    pose proof (term_in_preserving_lang_in_cmp _ _ _ _ pres_cmp H).
+    firstorder.
+    exists (map fst c').
+    exists x.
+    basic_core_crush.
+  }
+Qed.
 
-    all:repeat (erewrite compile_ctx_cmp_distributes;
-                [| | | eassumption | eassumption |];
-                [| basic_core_crush ..]).
+  
+Lemma wf_term_in_domain tgt cmp ir c e t
+  : preserving_compiler tgt cmp ir ->
+    wf_term ir c e t ->
+    term_in_cmp_domain cmp e.
+Proof.
+  intros; eapply wf_in_domain; eauto.
+Qed.
+#[export] Hint Resolve wf_term_in_domain : lang_core.
 
-    apply inductive_implies_semantic in pres_cmp'; firstorder.
-    
-    all: repeat (erewrite compile_sort_cmp_distributes;
-        [| | | eassumption | eassumption |];
-        [| basic_core_crush ..]).
-    
-    apply inductive_implies_semantic in pres_cmp'; firstorder.
-    
-    apply inductive_implies_semantic in pres_cmp'; firstorder.
-    all: repeat (erewrite compile_cmp_distributes;
-        [| | | eassumption | eassumption |];
-        [| basic_core_crush ..]).
-    
-    apply inductive_implies_semantic in pres_cmp'; firstorder.
-  Qed.
+Lemma wf_sort_in_domain tgt cmp ir c t
+  : preserving_compiler tgt cmp ir ->
+    wf_sort ir c t ->
+    sort_in_cmp_domain cmp t.
+Proof.
+  intros; eapply wf_in_domain; eauto.
+Qed.
+#[export] Hint Resolve wf_sort_in_domain : lang_core.
+
+Lemma wf_ctx_in_domain tgt cmp ir c
+  : preserving_compiler tgt cmp ir ->
+    wf_ctx ir c ->
+    all (sort_in_cmp_domain cmp) (map snd c).
+Proof.
+  induction 2; basic_goal_prep; basic_core_crush.
+Qed.
+#[export] Hint Resolve wf_ctx_in_domain : lang_core.
+  
+Lemma preserving_in_domain tgt cmp ir cmp' src
+  : preserving_compiler tgt cmp ir ->
+    preserving_compiler ir cmp' src ->
+    all (ccase_in_cmp_domain cmp) (map snd cmp').
+Proof.
+  intro pres_cmp.
+  induction 1; basic_goal_prep; intuition.
+  eapply wf_sort_in_domain; eauto.
+  eapply wf_term_in_domain; eauto.
+Qed.
+#[export] Hint Resolve preserving_in_domain : lang_core.
+  
+
+Theorem preservation_transitivity src ir tgt cmp cmp'
+  : wf_lang src ->
+    wf_lang ir ->
+    wf_lang tgt ->
+    preserving_compiler tgt cmp ir ->
+    preserving_compiler ir cmp' src ->
+    preserving_compiler tgt (compile_cmp cmp cmp') src.
+Proof using .
+  intros wfsrc wfir wftgt pres_cmp pres_cmp'.
+  pose proof (inductive_implies_semantic wfir wftgt pres_cmp).
+  firstorder.
+  revert wfsrc.
+  induction pres_cmp'; basic_goal_prep; constructor;
+    autorewrite with lang_core in *; firstorder eauto.
+  1,8,21,40:solve [apply inductive_implies_semantic in pres_cmp'; firstorder].
+  all: eauto with lang_core.
+  all: try match goal with [|- all_fresh _] => basic_core_crush end.
+  all: basic_core_crush.
+Qed.
+#[export] Hint Resolve preservation_transitivity : lang_core.
